Game.lean
@@ -1,4 +1,4 @@
-import Game.Levels.DemoWorld
+import Game.Levels.Preliminaries
 
 -- Here's what we'll put on the title screen
 Title "The Pumping Lemma Game"
@@ -6,7 +6,16 @@ Introduction
 "
 Welcome to the Pumping Lemma Game!
 
-In this game,
+In this game, we build a definition of a language in terms of formal languages. For this language,
+we prove various facts about appending two words or concating a character to a word, etc.
+These lemmas are then used to build the Pumping Lemma for regular languages.
+Finally, this Pumping Lemma is applied to some languages to show that those languages are not regular.
+
+This game should help you to dig deep into the definition of the Pumping Lemma. It should help you
+to understand the Pumping Lemma better by deriving several facts you might not think of when writing
+the proof on paper.
+
+Good luck and enjoy learning about the Pumping Lemma!
 "
 
 Info "
@@ -24,7 +33,9 @@ Warning: In most browsers, deleting cookies will also clear the local storage
 /-! Information to be displayed on the servers landing page. -/
 Languages "en"
 CaptionShort "A playful way to learn about the Pumping Lemma"
-CaptionLong "In this game, you prove some facts about formal languages and regular languages later on. Finally, you prove some facts about the Pumping Lemma and use them to prove that the language a^nb^n is not regular."
+CaptionLong "In this game, you prove some facts about the Language structure specifically defined
+for this game and later on other facts about the Pumping Lemma. Finally, you use these lemmas to
+prove that the provided examples fo languages are not regular languages."
 -- Prerequisites "" -- add this if your game depends on other games
 -- CoverImage "images/cover.png"
 
